theories/Core/Soundness/LogicalRelation/CoreTactics.v
@@ -29,7 +29,7 @@ Ltac invert_glu_rel1 :=
       progressive_invert H
   | H : sigma_glu_typ_pred _ _ _ _ _ _ _ |- _ =>
       progressive_invert H
-  | H : sigma_glu_exp_pred _ _ _ _ _ _ _ _ _ _ |- _ =>
+  | H : sigma_glu_exp_pred _ _ _ _ _ _ _ _ _ _ _ |- _ =>
       progressive_invert H
   | H : eq_glu_typ_pred _ _ _ _ _ _ _ |- _ =>
       progressive_invert H
